Add more examples for Aesop

tests/lean/AesopProblems.lean
@@ -12,11 +12,8 @@ namespace AesopProblems
   #
   #===========================================================================#-/
 
-/- A problem I have is that I often want to simplify expressions in the context, but
-   simplifying those expressions often requires something more powerful than [simp].
-
-   Below, all lemmas are written to represent minimal reproductions of goal states
-   which I encountered.
+/- I often encounter the situation where I want to simplify expressions in the context,
+   but simplifying those expressions often requires something more powerful than [simp].
  -/
 
 /- Here, I want to simplify the condition in the [if then else] (don't look at
@@ -30,17 +27,18 @@ namespace AesopProblems
 
    Of course, I'm aware that I can give to [simp] a tactic with which to solve
    the preconditions of the rewriting lemmas, but we can imagine more complex
-   settings where we actually want to apply rules, and solve the preconditions and
+   settings where we actually want to apply rules, and solve the preconditions of
    those rules with specific tactics, etc.
 
    Remark: I'm also aware that performance and stability of proofs which use [aesop] like
    a more powerful [simp] might be an issue, but I believe this is an orthogonal problem
    (and there are some immediate, though maybe sub-optimal solutions, like leverating the
-   fact that [aesop] can generate proof scripts).
+   fact that [aesop] can generate proof scripts to use [aesop] a bit like a copilot
+   in those situations).
 -/
 example (x : ℤ) (h : 0 ≤ x) :
-  if 0 ≤ x + 1 then ⊤
-  else ⊥ := by
+  if 0 ≤ x + 1 then ⊤ else ⊥
+  := by
   -- I have to write by hand this assertion, which then clutters the context,
   -- unless I clear it of course (another manual step)
   have : 0 ≤ x + 1 := by linarith
@@ -50,23 +48,23 @@ example (x : ℤ) (h : 0 ≤ x) :
 /- In the same spirit, I encountered this one a lot.
 
    When manipulating arrays (modeled as lists), we often find the following pattern, where
-   we access an access of an array from which we just updated an element. In this
-   situation we essentially use two lemmas, which give us that: if [update] and [index]
-   use the same index, then [index] evaluates to the updated element, otherwise [index]
-   evaluates to [index] of the old array.
+   we access an array from which we just updated an element. In this situation we
+   essentially use two lemmas, which give us that: if [update] and [index] use the same
+   index, then [index] evaluates to the updated element ([List.index_update_ne] in the
+   proof below), otherwise [index] evaluates to [index] of the old array ([List.index_update_eq]).
 
    Remark: in case you wonder, I have developed my own library of functions to
    manipulate lists so as never to use the type ℕ (I use ℤ instead) because
    proofs which mix ℤ and ℕ don't behave well. More details on that later.
  -/
 example (i j : ℤ) [Inhabited α] (l : List α) (x : α)
-  -- The fact that i ≠ j often comes from a set of (linear) equations
+  -- The fact that [i ≠ j] that we use below often comes from a set of (linear) equations
   (h1 : i + 1 ≤ j) :
   List.index (List.update l i x) j = List.index l j := by
-  -- The lemma we want to use has the precondition i ≠ j, which we have to assert by hand
+  -- The lemma we want to use has the precondition [i ≠ j], which we have to assert by hand
   have : i ≠ j := by scalar_tac -- [scalar_tac] is my "boosted" version of linarith
   -- We can finish with the simplifier (the lemma is actually marked as [simp],
-  -- so [simp [*]] would actually be enough.
+  -- so [simp [*]] would actually be enough).
   simp [List.index_update_ne, *]
 
 /- In case the indices are the same, we use the following lemma (which is also
@@ -77,8 +75,8 @@ example (i j : ℤ) [Inhabited α] (l : List α) (x : α)
    safe. The reason is that when we can apply [List.index_update_eq], the indices are
    often syntactically the same (or they are after a call to [simp]). This means that if
    [List.index (List.update l i x) j] doesn't get simplified to [x] because [i = j], it is
-   often safe to assume that we must have [i ≠ j] (and that if we don't manage to prove
-   that [i ≠ j] it simply means that we lack some information).
+   often safe to assume that we *must* have [i ≠ j] (and that if we don't manage to prove
+   [i ≠ j], it simply means that we lack some information in the context).
    But maybe this observation is too specific to the problem above...
  -/
 
@@ -130,11 +128,32 @@ example (i : ℤ) (l : List ℤ) (hi : ∀ i, 0 ≤ i → i < l.len → 0 < l.in
 example (x y : ℤ) (hx : 0 ≤ x) (hy : 0 ≤ y) : 0 ≤ x * y := by
   apply Left.mul_nonneg <;> assumption
 
+/- About non-linear arithmetic: I did some proofs about a hashmap and we are currently
+   working on the proof of the Kyber key encapsulation mechanism (it is a cryptographic
+   primitive), and we encounter(ed) a lot of issues because of non-linear arithmetic proof
+   obligations, which we think could be automated.
+
+   This includes a lot of things like proving [2 * x ≤ 2 * y] from [x ≤ y],
+   proving [x / d + y / d ≤ (x + y) / d], or that [(a * b) / c = a * (b / c)]
+   if [c | b] (and losing time because we need to find the proper lemma in
+   mathlib and we actually get confused because there are several definitions
+   of division: https://leanprover.zulipchat.com/#narrow/stream/287929-mathlib4/topic/efficiently.20dealing.20with.20.2F.20vs.20.2Ediv), etc.
+
+   I think this is the typical example where [aesop] would shine, because this
+   is a situation where we badly need some custom automation, but the automation
+   is not complex enough to justify writing a dedicated solver from scratch.
+   I would love to discuss this in more details (and get [aesop] to work on
+   those proofs!).
+ -/
+
 /- More generally speaking, I believe having sets of rules would really open
    the possibility of writing a wide range of specialized and quite efficient
-   solvers. For instance, for the problem above I would have [scalar_tac]
-   simply call [aesop] with the proper set of rules (also see the section
-   about the arithmetic tactics below).
+   solvers. For instance, for the problems above I would write a set of tactics
+   which simply call [aesop] with the proper set of rules (also see the section
+   about the arithmetic tactics below). One issue with the examples above is
+   that I am confident I can automate them with [aesop], but I would not
+   consider all the lemmas I want [aesop] to apply as safe to apply in a general
+   setting.
 
    About stability: marking theorems as rules for [aesop] looks a bit like a sophisticated
    version of SMT patterns. I guess you know what SMT patterns are, but just in case: with
@@ -148,14 +167,39 @@ example (x y : ℤ) (hx : 0 ≤ x) (hy : 0 ≤ y) : 0 ≤ x * y := by
 
 /-#===========================================================================#
   #
-  #     Automatic unfolding
+  #     Automatic unfolding of definitions
   #
   #===========================================================================#-/
 
-/- 
+/- I often have the following issue, where I want to unfold some definitions
+   (like an invariant), simplify the context at the same time, then call a tactic
+   like [scalar_tac].
 
+   At a high level, I would like to be able to write something like what
+   people do in Dafny:
+   ```
+   reveal(inv);
+   ```
+
+   or:
+   ```
+   assert ... by { reveal(inv) }
+   ```
+
+   This is also another motivation to have the possibility of defining sets
+   of rules.
+
+   Remark: I think [aesop] can easily handle this problem already. I mostly wanted to
+   mention it, because it is something I often encounter.
  -/
 
+def inv (ls : List ℤ) : Prop := 0 < ls.len
+
+example (ls : List ℤ) (hinv : inv ls) : 1 ≤ ls.len := by
+  simp_all [inv]
+  scalar_tac
+
+/- Remark: unfolding definitions is of course not limited to unfolding invariants. -/
 
 /-#===========================================================================#
   #
@@ -163,8 +207,74 @@ example (x y : ℤ) (hx : 0 ≤ x) (hy : 0 ≤ y) : 0 ≤ x * y := by
   #
   #===========================================================================#-/
 
-/- 
+/- I mentioned the fact that I wrote my own library of functions to operate on
+   lists, in order never to use ℕ (always ℤ), because proofs which mix ℤ and ℕ
+   are tedious.
 
+   The main issue comes from the fact that, if we want to call linarith
+   on a goal, we need to convert all the ℕ to ℤ. We can do so by calling
+   [zify] and the simplifier, expect when we have substrations.
+   Indeed, we have [↑(x - y) = ↑x - ↑y] (where x, y ∈ ℕ) only if we can prove
+   that [y ≤ x]. I wonder how [aesop] could help us with that.
+
+   Also, my [scalar_tac] could probably be implemented on top of [aesop].
+   It does the following:
+   - introduces the bounds for the machine integers (and some other bounds,
+     like [0 ≤ l.len] if [l] is a list in the context - note that [List.len]
+     is my custom version of [List.length], which returns an [ℤ]). I implemented
+     this with typeclasses (I explore the goal, and lookup instances of a specific
+     typeclass for all the subterms - it works well in practice).
+   - splits on occurrences of [x ≠ y] (because last time I looked it was not
+     implemented yet for [linarith]
+   - performs a very controled simplification of the context
  -/
+
+example (x : U32) (ls : List α) : 0 ≤ x.val + ls.len := by
+  -- This is the preprocessing performed by [scalar_tac], just to show
+  -- you what we get.
+  --
+  -- Side note: you may wonder why we introduce assumptions like: [4294967295 ≤ Usize.max].
+  -- This is because as [Usize.max] depends on the architecture, we make it opaque.
+  scalar_tac_preprocess
+  -- Finishing off the proof
+  linarith
+
+/-#===========================================================================#
+  #
+  #     Not completely related: matching terms with a database of theorems
+  #
+  #===========================================================================#-/
+
+/- I showed you the [progress] tactic (see example below), which allows to do Hoare-style
+   proofs on functions written in an error monad. It works by looking at the goal, looking
+   up a theorem (among the theorems we marked with a dedicated attribute) which matches
+   the first function call, and applying it.
+
+   I had to implement my own lookup function, which is not very powerful (I map
+   function *names* to theorems). It works in most situations, but not when
+   we use typeclasses. For instance, I have theorems for operations like [x + y],
+   which desugars to [HAdd.hAdd (Scalar ...) x y]. I can't simply map [HAdd.hAdd]
+   to the theorem I need because it depends on the type (second argument).
+   For now I have a workaround, but I'm not very satisfied with it. I would like to have
+   something which gives me all the theorems which match a given term.
+
+   So my question is: what I need is actually similar to what [simp] and [aesop] must
+   themselves do. Is there some code in [simp] or [aesop] that I could reuse for this
+   purpose?
+ -/
+
+def mul2_add1 (x : U32) : Result U32 := do
+  let x1 ← x + x
+  let x2 ← x1 + 1#u32
+  ret x2
+
+theorem mul2_add1_spec2 (x : U32) (h : 2 * ↑x + 1 ≤ U32.max)
+  : ∃ y, mul2_add1 x = ret y ∧
+  ↑ y = 2 * ↑x + (1 : Int)
+  := by
+  rw [mul2_add1]
+  progress as ⟨ x1 .. ⟩ -- we progress by one step in the goal
+  progress as ⟨ x2 .. ⟩
+  simp at *; scalar_tac
 
 end AesopProblems
